examples/base-src/manual/GHC/IO.v
@@ -1,0 +1,94 @@
+Require Import GHC.Base.
+
+Inductive Freer (E : Type -> Type) (R : Type) :=
+| Ret (r : R)
+| Vis (X : Type) (e : E X) (k : X -> Freer E R).
+
+Arguments Ret {_} {_}.
+Arguments Vis {_} {_} {_}.
+
+Set Implicit Arguments.
+
+Section IO.
+
+  Variable E : Type -> Type.
+  Variables X Y : Type.
+
+  Fixpoint bind (a : Freer E X) (f : X -> Freer E Y) : Freer E Y :=
+    match a with
+    | Ret x => f x
+    | Vis e k => Vis e (fun x => bind (k x) f)
+    end.
+
+  Definition ret (a : X) : Freer E X := Ret a.
+
+  Definition vis (m: E X) : Freer E X := Vis m (fun x => Ret x).
+
+  Definition mask_ (x : Freer E X) : Freer E X := x.
+
+  Definition onException (x : Freer E X) (y : Freer E Y) : Freer E X := x.
+
+End IO.
+
+Arguments ret {_} {_}.
+Arguments vis {_} {_}.
+
+Section IOMonad.
+
+  Variable E : Type -> Type.
+
+  Local Definition Functor__IO_fmap
+    : forall {a} {b}, (a -> b) -> Freer E a -> Freer E b :=
+    fun {a} {b} f x => bind x (fun y => ret (f y)).
+
+  Local Definition Functor__IO_op_zlzd__
+    : forall {a} {b}, a -> Freer E b -> Freer E a :=
+    fun {a} {b} => Functor__IO_fmap ∘ const.
+
+  Program Instance Functor__IO : Functor (Freer E) :=
+    fun _ k =>
+      k {| fmap__ := fun {a} {b} => Functor__IO_fmap;
+           op_zlzd____ := fun {a} {b} => Functor__IO_op_zlzd__ |}.
+
+  Local Definition Applicative__IO_op_zlztzg__
+    : forall {a} {b}, Freer E (a -> b) -> Freer E a -> Freer E b :=
+    fun {a} {b} =>
+      fun fs xs => bind fs (fun f => bind xs (fun x => ret (f x))).
+
+  Local Definition Applicative__IO_liftA2
+    : forall {a} {b} {c}, (a -> b -> c) -> Freer E a -> Freer E b -> Freer E c :=
+    fun {a} {b} {c} =>
+      fun f xs ys => Applicative__IO_op_zlztzg__ (Functor__IO_fmap f xs) ys.
+
+  Local Definition Applicative__IO_op_ztzg__
+    : forall {a} {b}, Freer E a -> Freer E b -> Freer E b :=
+    fun {a} {b} =>
+      fun xs ys => Applicative__IO_op_zlztzg__ (Functor__IO_op_zlzd__ (fun x => x) xs) ys.
+
+  Local Definition Applicative__IO_pure : forall {a}, a -> Freer E a :=
+    fun {a} => ret.
+
+  Program Instance Applicative__IO : Applicative (Freer E) :=
+    fun _ k =>
+      k {| liftA2__ := fun {a} {b} {c} => Applicative__IO_liftA2 ;
+           op_zlztzg____ := fun {a} {b} => Applicative__IO_op_zlztzg__ ;
+           op_ztzg____ := fun {a} {b} => Applicative__IO_op_ztzg__ ;
+           pure__ := fun {a} => Applicative__IO_pure |}.
+  
+  Local Definition Monad__IO_return_ : forall {a}, a -> Freer E a :=
+    fun {a} => pure.
+
+  Local Definition Monad__IO_op_zgzg__
+    : forall {a} {b}, Freer E a -> Freer E b -> Freer E b :=
+    fun {a} {b} => _*>_.
+
+  Local Definition Monad__IO_op_zgzgze__
+    : forall {a} {b}, Freer E a -> (a -> Freer E b) -> Freer E b :=
+    fun {a} {b} => @bind E a b.
+  
+  Program Instance Monad__IO : Monad (Freer E) :=
+    fun _ k =>
+      k {| op_zgzg____ := fun {a} {b} => Monad__IO_op_zgzg__ ;
+           op_zgzgze____ := fun {a} {b} => Monad__IO_op_zgzgze__ ;
+           return___ := fun {a} => Monad__IO_return_ |}.
+End IOMonad.
